src/program_proof/tulip/paxos/program/paxos.v
@@ -73,34 +73,27 @@ Section repr.
       "HconnsP"     ∷ paxos ↦[Paxos :: "conns"] #connsP ∗
       "#Hpeers"     ∷ own_slice peersP uint64T DfracDiscarded (elements peers).
 
-  Definition own_paxos_votes
-    (termc termp : u64) (entsc entsp : list string) (respp : gmap u64 bool) γ : iProp Σ :=
-    ∃ (dss : gmap u64 (list nodedec)),
-      "#Hdss"      ∷ ([∗ map] nid↦ds ∈ dss, is_past_nodedecs_lb γ nid ds) ∗
-      "%Hlendss"   ∷ ⌜map_Forall (λ _ ds, (length ds = uint.nat termc)%nat) dss⌝ ∗
-      "%Hlatestq"  ∷ ⌜latest_term_before_quorum_nodedec dss (uint.nat termc) = (uint.nat termp)⌝ ∗
-      "%Hlongestq" ∷ ⌜longest_proposal_in_term_nodedec dss (uint.nat termp) = Some (entsc ++ entsp)⌝ ∗
-      "%Hrspd"     ∷ ⌜dom dss = dom respp⌝.
-
   Definition own_paxos_candidate_only
-    (nidme termc terml termp : u64) (entsc : list string)
-    (entspP : Slice.t) (resppP : loc) γ : iProp Σ :=
+    (nidme termc terml termp : u64) (logc : list string)
+    (entspP : Slice.t) (resppP : loc) nids γ : iProp Σ :=
     ∃ (entsp : list string) (respp : gmap u64 bool),
       "Hentsp"    ∷ own_slice entspP stringT (DfracOwn 1) entsp ∗
       "Hrespp"    ∷ own_map resppP (DfracOwn 1) respp ∗
-      "#Hvotes"   ∷ own_paxos_votes termc termp entsc entsp respp γ ∗
+      "#Hvotes"   ∷ votes_in γ (dom respp) (uint.nat termc) (uint.nat termp) (logc ++ entsp) ∗
       "%Hton"     ∷ ⌜is_term_of_node nidme (uint.nat termc)⌝ ∗
-      "%Hlcne"    ∷ ⌜uint.Z terml ≠ uint.Z termc⌝.
+      "%Hdomvts"  ∷ ⌜dom respp ⊆ nids⌝ ∗
+      "%Hllep"    ∷ ⌜uint.Z terml ≤ uint.Z termp⌝ ∗
+      "%Hpltc"    ∷ ⌜uint.Z termp < uint.Z termc⌝.
 
   Definition own_paxos_candidate
-    (paxos : loc) (nid termc terml : u64) (entsc : list string) (iscand : bool) γ : iProp Σ :=
+    (paxos : loc) (nid termc terml : u64) (entsc : list string) (iscand : bool) nids γ : iProp Σ :=
     ∃ (termp : u64) (entspP : Slice.t) (resppP : loc),
       "HiscandP" ∷ paxos ↦[Paxos :: "iscand"] #iscand ∗
       "HtermpP"  ∷ paxos ↦[Paxos :: "termp"] #termp ∗
       "HentspP"  ∷ paxos ↦[Paxos :: "entsp"] (to_val entspP) ∗
       "HresppP"  ∷ paxos ↦[Paxos :: "respp"] #resppP ∗
       "Honlyc"   ∷ (if iscand
-                    then own_paxos_candidate_only nid termc terml termp entsc entspP resppP γ
+                    then own_paxos_candidate_only nid termc terml termp entsc entspP resppP nids γ
                     else True).
 
   Definition own_paxos_leader_only (termc : u64) (ents : list string) γ : iProp Σ :=
@@ -139,6 +132,9 @@ Section repr.
       "Hsafecmt"   ∷ safe_ledger_above γ nids (uint.nat terml) (take (uint.nat lsnc) log) ∗ 
       "Hcomm"      ∷ own_paxos_comm paxos peers ∗
       "Hsc"        ∷ own_paxos_sc paxos nids ∗
+      "#Hpreped"   ∷ (if decide (termc = terml)
+                      then True
+                      else past_nodedecs_latest_before γ nidme (uint.nat termc) (uint.nat terml) log) ∗
       "%Hnids"     ∷ ⌜nids = {[nidme]} ∪ peers⌝ ∗
       "%Hnid"      ∷ ⌜0 ≤ uint.Z nidme < max_nodes⌝ ∗
       "%Htermlc"   ∷ ⌜uint.Z terml ≤ uint.Z termc⌝ ∗
@@ -150,40 +146,47 @@ Section repr.
   that are decomposed (e.g., [terml]) into smaller pieces of representation
   predicates should be existentially quantified. *)
   Definition own_paxos_internal
-    (paxos : loc) (termc lsnc : u64) (iscand isleader : bool) nids γ : iProp Σ :=
-    ∃ (nidme terml : u64) (log : list string),
+    (paxos : loc) (nidme termc terml lsnc : u64) (iscand isleader : bool) nids γ : iProp Σ :=
+    ∃ (log : list string),
       let logc := (take (uint.nat lsnc) log) in
       "Hpx"     ∷ own_paxos_common paxos nidme termc terml lsnc log nids γ ∗
-      "Hcand"   ∷ own_paxos_candidate paxos nidme termc terml logc iscand γ ∗
+      "Hcand"   ∷ own_paxos_candidate paxos nidme termc terml logc iscand nids γ ∗
       "Hleader" ∷ own_paxos_leader paxos termc log isleader γ.
 
   Definition own_paxos_with_termc_lsnc
-    (paxos : loc) (termc lsnc : u64) nids γ : iProp Σ :=
-    ∃ (iscand : bool) (isleader : bool),
-      own_paxos_internal paxos termc lsnc iscand isleader nids γ.
+    (paxos : loc) (nidme termc lsnc : u64) nids γ : iProp Σ :=
+    ∃ (terml : u64) (iscand isleader : bool),
+      own_paxos_internal paxos nidme termc terml lsnc iscand isleader nids γ.
 
   Definition own_paxos_nominiated_with_termc_lsnc
-    (paxos : loc) (termc lsnc : u64) nids γ : iProp Σ :=
-    ∃ (isleader : bool),
-      own_paxos_internal paxos termc lsnc true isleader nids γ.
+    (paxos : loc) (nidme termc lsnc : u64) nids γ : iProp Σ :=
+    ∃ (terml : u64) (isleader : bool),
+      own_paxos_internal paxos nidme termc terml lsnc true isleader nids γ.
 
   Definition own_paxos_with_termc
-    (paxos : loc) (termc : u64) nids γ : iProp Σ :=
+    (paxos : loc) (nidme termc : u64) nids γ : iProp Σ :=
+    ∃ (terml lsnc : u64) (iscand : bool) (isleader : bool),
+      own_paxos_internal paxos nidme termc terml lsnc iscand isleader nids γ.
+
+  Definition own_paxos_with_termc_terml
+    (paxos : loc) (nidme termc terml : u64) nids γ : iProp Σ :=
     ∃ (lsnc : u64) (iscand : bool) (isleader : bool),
-      own_paxos_internal paxos termc lsnc iscand isleader nids γ.
+      own_paxos_internal paxos nidme termc terml lsnc iscand isleader nids γ.
 
-  Definition own_paxos (paxos : loc) nids γ : iProp Σ :=
-    ∃ (termc lsnc : u64) (iscand : bool) (isleader : bool),
-      own_paxos_internal paxos termc lsnc iscand isleader nids γ.
+  Definition own_paxos (paxos : loc) (nidme : u64) nids γ : iProp Σ :=
+    ∃ (termc terml lsnc : u64) (iscand : bool) (isleader : bool),
+      own_paxos_internal paxos nidme termc terml lsnc iscand isleader nids γ.
 
-  Definition own_paxos_nominated (paxos : loc) nids γ : iProp Σ :=
-    ∃ (termc lsnc : u64) (isleader : bool),
-      own_paxos_internal paxos termc lsnc true isleader nids γ.
+  Definition own_paxos_nominated (paxos : loc) (nidme : u64) nids γ : iProp Σ :=
+    ∃ (termc terml lsnc : u64) (isleader : bool),
+      own_paxos_internal paxos nidme termc terml lsnc true isleader nids γ.
 
-  Definition is_paxos (paxos : loc) γ : iProp Σ :=
+  (* TODO: finding the right states to expose after adding network. *)
+
+  Definition is_paxos (paxos : loc) (nidme : u64) γ : iProp Σ :=
     ∃ (mu : loc) (nids : gset u64),
       "#HmuP"  ∷ readonly (paxos ↦[Paxos :: "mu"] #mu) ∗
-      "#Hlock" ∷ is_lock paxosNS #mu (own_paxos paxos nids γ) ∗
+      "#Hlock" ∷ is_lock paxosNS #mu (own_paxos paxos nidme nids γ) ∗
       "#Hinv"  ∷ know_paxos_inv γ nids.
 
 End repr.
@@ -191,12 +194,12 @@ End repr.
 Section stepdown.
   Context `{!heapGS Σ, !paxos_ghostG Σ}.
 
-  Theorem wp_Paxos__stepdown px (term : u64) termc nids γ :
+  Theorem wp_Paxos__stepdown px (nidme term : u64) termc nids γ :
     uint.Z termc < uint.Z term ->
     know_paxos_inv γ nids -∗
-    {{{ own_paxos_with_termc px termc nids γ }}}
+    {{{ own_paxos_with_termc px nidme termc nids γ }}}
       Paxos__stepdown #px #term
-    {{{ RET #(); own_paxos_with_termc px term nids γ }}}.
+    {{{ RET #(); own_paxos_with_termc px nidme term nids γ }}}.
   Proof.
     iIntros (Hlt) "#Hinv".
     iIntros (Φ) "!> Hpx HΦ".
@@ -223,7 +226,9 @@ Section stepdown.
     iApply "HΦ".
     iFrame "HiscandP".
     assert (Htermlc' : uint.Z terml ≤ uint.Z term) by word.
-    by iFrame "∗ # %".
+    iFrame "∗ # %".
+    iClear "Hpreped".
+    by case_decide.
   Qed.
 
 End stepdown.
@@ -231,11 +236,11 @@ End stepdown.
 Section nominate.
   Context `{!heapGS Σ, !paxos_ghostG Σ}.
 
-  Theorem wp_Paxos__nominate (px : loc) nids γ :
+  Theorem wp_Paxos__nominate (px : loc) (nidme : u64) nids γ :
     know_paxos_inv γ nids -∗
-    {{{ own_paxos px nids γ }}}
+    {{{ own_paxos px nidme nids γ }}}
       Paxos__nominate #px
-    {{{ (term : u64) (lsn : u64), RET (#term, #lsn); own_paxos px nids γ }}}.
+    {{{ (term : u64) (lsn : u64), RET (#term, #lsn); own_paxos px nidme nids γ }}}.
   Proof.
     iIntros "#Hinv" (Φ) "!> Hpx HΦ".
     wp_rec. wp_pures.
@@ -312,7 +317,8 @@ Section nominate.
     assert (Hlcne' : uint.Z terml ≠ uint.Z term) by word.
     set logc := take _ log.
     set entsp := drop _ log.
-    iAssert (own_paxos_votes term terml logc entsp {[nidme := true]} γ)%I as "Hvotes".
+    set respp' := map_insert _ _ _.
+    iAssert (votes_in γ (dom respp') (uint.nat term) (uint.nat terml) (logc ++ entsp))%I as "Hvotes".
     { iNamed "Hpromise".
       iExists {[nidme := ds]}.
       rewrite big_sepM_singleton.
@@ -325,13 +331,21 @@ Section nominate.
         by rewrite -latest_term_before_nodedec_unfold -Hlends -latest_term_nodedec_unfold.
       }
       split.
-      { apply longest_proposal_in_term_with_singleton.
+      { apply length_of_longest_ledger_in_term_singleton.
         by rewrite Hacpt take_drop.
       }
-      { by rewrite 2!dom_singleton_L. }
+      split.
+      { by rewrite map_Exists_singleton Hacpt take_drop. }
+      { rewrite dom_singleton_L dom_insert_L. set_solver. }
     }
     iFrame "HiscandP HisleaderP".
-    by iFrame "∗ # %".
+    iFrame "∗ # %".
+    iModIntro.
+    iSplit.
+    { iClear "Hpreped". by case_decide. }
+    iPureIntro.
+    split; last lia.
+    rewrite dom_insert_L. set_solver.
   Qed.
 
 End nominate.
@@ -351,39 +365,116 @@ Section cquorum.
 
 End cquorum.
 
-Section collect.
+Section lemma.
   Context `{!paxos_ghostG Σ}.
-    
-  
-End collect.
+
+  Lemma node_inv_past_nodedecs_impl_prefix_base_ledger γ nid ds dslb psa t v :
+    dslb !! t = Some (Accept v) ->
+    is_past_nodedecs_lb γ nid dslb -∗
+    node_inv_ds_psa γ nid ds psa -∗
+    prefix_base_ledger γ t v.
+  Proof.
+    iIntros (Hv) "Hdslb Hnode".
+    iNamed "Hnode". iNamed "Hpsa".
+    iDestruct (past_nodedecs_prefix with "Hdslb Hpastd") as %Hprefix.
+    pose proof (prefix_lookup_Some _ _ _ _ Hv Hprefix) as Hdst.
+    specialize (Hfixed _ _ Hdst).
+    by iDestruct (big_sepM_lookup with "Hpsalbs") as "?"; first apply Hfixed.
+  Qed.
+
+  Lemma safe_ledger_past_nodedecs_impl_prefix γ nids nid dslb t1 t2 v1 v2 :
+    nid ∈ nids ->
+    (t1 < t2)%nat ->
+    dslb !! t2 = Some (Accept v2) ->
+    safe_ledger_in γ nids t1 v1 -∗
+    is_past_nodedecs_lb γ nid dslb -∗
+    paxos_inv γ nids -∗
+    ⌜prefix v1 v2⌝.
+  Proof.
+    iIntros (Hnid Hlt Hv2) "Hsafev1 Hdslb Hinv".
+    iNamed "Hinv".
+    iDestruct (nodes_inv_extract_ds_psa with "Hnodes") as (dss bs) "[Hndp Hnodes]".
+    (* Obtain [dom termlm = dom bs]. *)
+    iDestruct (big_sepM2_dom with "Hnodes") as %Hdomdp.
+    iDestruct (big_sepM2_dom with "Hndp") as %Hdom.
+    rewrite dom_map_zip_with_L Hdomdp intersection_idemp_L Hdomtermlm in Hdom.
+    symmetry in Hdom.
+    iClear "Hndp".
+    (* Obtain [prefix_base_ledger γ t2 v2]. *)
+    iAssert (prefix_base_ledger γ t2 v2)%I as (vb) "[#Hvb %Hvblev2]".
+    { assert (is_Some (dss !! nid)) as [ds Hds].
+      { by rewrite -elem_of_dom Hdomdp Hdom. }
+      assert (is_Some (bs !! nid)) as [psa Hpsa].
+      { by rewrite -elem_of_dom Hdom. }
+      iDestruct (big_sepM2_lookup with "Hnodes") as "Hnode"; [apply Hds | apply Hpsa |].
+      by iApply (node_inv_past_nodedecs_impl_prefix_base_ledger with "Hdslb Hnode").
+    }
+    (* Obtain [valid_base_proposals], [valid_lb_ballots], and [valid_ub_ballots]. *)
+    iDestruct (nodes_inv_impl_valid_base_proposals with "Hsafepsb Hnodes") as %Hvbp.
+    { apply Hdom. }
+    iDestruct (nodes_inv_ds_psa_impl_nodes_inv_psa with "Hnodes") as "Hnodes".
+    iDestruct (nodes_inv_impl_valid_lb_ballots with "Hpsb Hnodes") as %Hvlb.
+    iDestruct (nodes_inv_impl_valid_ub_ballots with "Hps Hnodes") as %Hvub.
+    (* Obtain [proposed_after_chosen] from the above. *)
+    pose proof (vlb_vub_vbp_impl_pac _ _ _ Hvlb Hvub Hvbp) as Hpac.
+    (* Obtain [chosen_in bs p v1] *)
+    iDestruct (nodes_inv_safe_ledger_in_impl_chosen_in with "Hsafev1 Hnodes") as %Hchosen.
+    { apply Hdom. }
+    (* Obtain [psb !! t2 = Some vb]. *)
+    iDestruct (base_proposal_lookup with "Hvb Hpsb") as %Hvb.
+    iPureIntro.
+    specialize (Hpac _ _ _ _ Hlt Hchosen Hvb).
+    by trans vb.
+  Qed.
+
+End lemma.
 
 Section collect.
   Context `{!heapGS Σ, !paxos_ghostG Σ}.
 
   Theorem wp_Paxos__collect
     (px : loc) (nid : u64) (term : u64)
-    (entsP : Slice.t) (ents : list string)
+    (nidme : u64) (entsP : Slice.t) (ents : list string)
     (termc lsnc : u64) (logpeer : list string) nids γ :
+    nid ∈ nids ->
     drop (uint.nat lsnc) logpeer = ents ->
     past_nodedecs_latest_before γ nid (uint.nat termc) (uint.nat term) logpeer -∗
-    {{{ own_paxos_nominiated_with_termc_lsnc px termc lsnc nids γ ∗
+    know_paxos_inv γ nids -∗
+    {{{ own_paxos_nominiated_with_termc_lsnc px nidme termc lsnc nids γ ∗
         own_slice entsP stringT (DfracOwn 1) ents
     }}}
       Paxos__collect #px #nid #term (to_val entsP)
-    {{{ RET #(); own_paxos_nominated px nids γ }}}.
+    {{{ RET #(); own_paxos_nominated px nidme nids γ }}}.
   Proof.
-    iIntros (Hlogpeer) "#Hpromise".
-    iIntros (Φ) "!> [Hpx Hentspeer] HΦ".
+    iIntros (Hinnids Hlogpeer) "#Hpromise #Hinv".
+    iIntros (Φ) "!> [Hpx Hents] HΦ".
     wp_rec. wp_pures.
 
     (*@ func (px *Paxos) collect(nid uint64, term uint64, ents []string) {      @*)
+    (*@     _, recved := px.respp[nid]                                          @*)
+    (*@     if recved {                                                         @*)
+    (*@         // Vote from [nid] has already been received.                   @*)
+    (*@         return                                                          @*)
+    (*@     }                                                                   @*)
+    (*@                                                                         @*)
+    iNamed "Hpx". iNamed "Hcand". iNamed "Honlyc".
+    wp_loadField.
+    wp_apply (wp_MapGet with "Hrespp").
+    iIntros (v recved) "[%Hrecved Hrespp]".
+    wp_if_destruct.
+    { iApply "HΦ".
+      iFrame "Hpx HentspP HiscandP".
+      by iFrame "∗ # %".
+    }
+    apply map_get_false in Hrecved as [Hrecved _].
+    clear Heqb v recved.
+
     (*@     if term < px.termp {                                                @*)
     (*@         // Simply record the response if the peer has a smaller term.   @*)
     (*@         px.respp[nid] = true                                            @*)
     (*@         return                                                          @*)
     (*@     }                                                                   @*)
     (*@                                                                         @*)
-    iNamed "Hpx". iNamed "Hcand". iNamed "Honlyc".
     wp_loadField.
     wp_if_destruct.
     { wp_loadField.
@@ -392,7 +483,8 @@ Section collect.
       wp_pures.
       iApply "HΦ".
       set logc := take _ log.
-      iAssert (own_paxos_votes termc termp logc entsp (<[nid := true]> respp) γ)%I
+      set respp' := map_insert _ _ _.
+      iAssert (votes_in γ (dom respp') (uint.nat termc) (uint.nat termp) (logc ++ entsp))%I
         as "Hvotes'".
       { iNamed "Hpromise".
         iNamed "Hvotes".
@@ -402,14 +494,37 @@ Section collect.
         split.
         { by apply map_Forall_insert_2. }
         split.
-        { admit. }
+        { rewrite /latest_term_before_quorum_nodedec.
+          rewrite (latest_term_before_quorum_with_insert_le _ _ _ _ _ (uint.nat term)).
+          { done. }
+          { by rewrite -not_elem_of_dom -Hdomdss not_elem_of_dom. }
+          { rewrite -Hlends. apply Hlatest. }
+          rewrite -latest_term_before_quorum_nodedec_unfold Hlatestq.
+          clear -Heqb.
+          word.
+        }
         split.
-        { admit. }
-        { by rewrite 2!dom_insert_L Hrspd. }
+        { rewrite length_of_longest_ledger_in_term_insert_None; first apply Hlongestq.
+          { by rewrite -not_elem_of_dom -Hdomdss not_elem_of_dom. }
+          rewrite (latest_term_before_with_None (mbind nodedec_to_ledger) (length ds)).
+          { done. }
+          rewrite /latest_term_nodedec /latest_term_before_nodedec in Hlatest.
+          word.
+        }
+        split.
+        { apply map_Exists_insert_2_2; last done.
+          by rewrite -not_elem_of_dom -Hdomdss not_elem_of_dom.
+        }
+        { by rewrite 2!dom_insert_L Hdomdss. }
       }
       iFrame "Hpx HentspP HiscandP".
-      by iFrame "∗ # %".
+      iFrame "∗ # %".
+      iPureIntro.
+      rewrite dom_insert_L.
+      set_solver.
     }
+    rewrite Z.nlt_ge in Heqb.
+    rename Heqb into Htermple.
 
     (*@     if term == px.termp && uint64(len(ents)) <= uint64(len(px.entsp)) { @*)
     (*@         // Simply record the response if the peer has the same term, but not @*)
@@ -432,15 +547,64 @@ Section collect.
     }
     iNamed 1.
     wp_if_destruct.
-    { wp_loadField.
+    { destruct Heqb as [Heq Hszle].
+      inv Heq.
+      iDestruct (own_slice_sz with "Hents") as %Hszents.
+      iDestruct (own_slice_sz with "Hentsp") as %Hszentsp.
+      wp_loadField.
       wp_apply (wp_MapInsert with "Hrespp"); first done.
       iIntros "Hrespp".
       wp_pures.
       iApply "HΦ".
+      set logc := take _ log.
+      set respp' := map_insert _ _ _.
+      iAssert (⌜uint.Z lsnc ≤ length log⌝)%I as %Hlsncub.
+      { by iNamed "Hpx". }
+      iAssert (votes_in γ (dom respp') (uint.nat termc) (uint.nat termp) (logc ++ entsp))%I
+        as "Hvotes'".
+      { iNamed "Hpromise".
+        iNamed "Hvotes".
+        iDestruct (big_sepM_insert_2 with "Hpastd Hdss") as "Hdss'".
+        iFrame "Hdss'".
+        iPureIntro.
+        split.
+        { by apply map_Forall_insert_2. }
+        split.
+        { rewrite /latest_term_before_quorum_nodedec.
+          rewrite (latest_term_before_quorum_with_insert_le _ _ _ _ _ (uint.nat termp)).
+          { done. }
+          { by rewrite -not_elem_of_dom -Hdomdss not_elem_of_dom. }
+          { rewrite -Hlends. apply Hlatest. }
+          rewrite -latest_term_before_quorum_nodedec_unfold Hlatestq.
+          done.
+        }
+        split.
+        { rewrite (length_of_longest_ledger_in_term_insert_Some_length_le _ _ _ _ logpeer).
+          { apply Hlongestq. }
+          { by rewrite -not_elem_of_dom -Hdomdss not_elem_of_dom. }
+          { by rewrite Hacpt. }
+          rewrite length_drop in Hszents.
+          rewrite Hlongestq length_app length_take.
+          clear -Hszents Hszentsp Hszle Hlsncub.
+          word.
+        }
+        split.
+        { apply map_Exists_insert_2_2; last done.
+          by rewrite -not_elem_of_dom -Hdomdss not_elem_of_dom.
+        }
+        { by rewrite 2!dom_insert_L Hdomdss. }
+      }
       iFrame "Hpx HiscandP".
       iFrame "∗ # %".
-      admit.
+      iPureIntro.
+      rewrite dom_insert_L.
+      set_solver.
     }
+    apply Classical_Prop.not_and_or in Heqb.
+    rename Heqb into Hcase.
+    rewrite Z.nle_gt in Hcase.
+    iDestruct (own_slice_sz with "Hents") as %Hszents.
+    iDestruct (own_slice_sz with "Hentsp") as %Hszentsp.
 
     (*@     // Update the largest term and longest log seen so far in this preparing @*)
     (*@     // phase, and record the response.                                  @*)
@@ -452,18 +616,149 @@ Section collect.
     wp_loadField.
     wp_apply (wp_MapInsert with "Hrespp"); first done.
     iIntros "Hrespp".
-  Admitted.
+    wp_pures.
+    iApply "HΦ".
+    set logc := take _ log.
+    set respp' := map_insert _ _ _.
+    iAssert (⌜uint.Z term < uint.Z termc⌝)%I as %Htermlt.
+    { iNamed "Hpromise".
+      iPureIntro.
+      rewrite /latest_term_nodedec /latest_term_before_nodedec Hlends in Hlatest.
+      set f := mbind _ in Hlatest.
+      unshelve epose proof (latest_term_before_with_lt f (uint.nat termc) ds _) as Hlt.
+      { word. }
+      clear -Hlt Hlatest.
+      word.
+    }
+    (* Prove that the committed part [logc] matches on the leader and peer sides. *)
+    iInv "Hinv" as "> HinvO" "HinvC".
+    iAssert (⌜logpeer = logc ++ ents⌝)%I as %->.
+    { (* Obtain [safe_ledger_above]. *)
+      iNamed "Hpx".
+      iDestruct "Hsafecmt" as (p) "[Hsafecmt %Hple]".
+      iNamed "Hpromise".
+      destruct (decide (p < uint.nat term)%nat) as [Hlt | Hge].
+      { iDestruct (safe_ledger_past_nodedecs_impl_prefix with "Hsafecmt Hpastd HinvO") as %Hlogc.
+        { apply Hinnids. }
+        { apply Hlt. }
+        { apply Hacpt. }
+        iPureIntro.
+        subst logc.
+        rewrite -(take_drop (uint.nat lsnc) logpeer) -Hlogpeer.
+        f_equal.
+        destruct Hlogc as [logtail ->].
+        rewrite take_app_le; last first.
+        { rewrite length_take. clear -Hlsncub. lia. }
+        by rewrite take_idemp.
+      }
+      assert (term = termp) as ->.
+      { clear -Hple Hge Htermple Hllep. word. }
+      destruct Hcase as [? | Hlenlt]; first done.
+      assert (p = uint.nat termp) as ->.
+      { clear -Hple Hge Htermple Hllep. lia. }
+      iDestruct "Hsafecmt" as (nidx nidsq) "Hsafecmt".
+      iNamed "Hsafecmt".
+      iDestruct (paxos_inv_impl_nodes_inv with "HinvO") as (termlm) "[Hnodes %Hdomtermlm]".
+      iDestruct (nodes_inv_extract_ds_psa with "Hnodes") as (dss bs) "[Hndp Hnodes]".
+      iDestruct (big_sepM2_dom with "Hnodes") as %Hdomdp.
+      iDestruct (big_sepM2_dom with "Hndp") as %Hdom.
+      rewrite dom_map_zip_with_L Hdomdp intersection_idemp_L Hdomtermlm in Hdom.
+      symmetry in Hdom.
+      iClear "Hndp".
+      iDestruct (accepted_proposal_past_nodedecs_impl_prefix with "Hvacpt Hpastd Hnodes")
+        as %Horprefix.
+      { rewrite Hdom. apply Hmember. }
+      { rewrite Hdom. apply Hinnids. }
+      { apply Hacpt. }
+      iPureIntro.
+      assert (Hlogc : prefix logc logpeer).
+      { destruct Horprefix as [Hprefix | Hprefix]; first apply Hprefix.
+        rewrite (prefix_length_eq _ _ Hprefix); first done.
+        rewrite length_take.
+        unshelve epose proof (drop_lt_inv logpeer (uint.nat lsnc) _) as Hgt.
+        { rewrite Hlogpeer. intros ->. simpl in Hszents. clear -Hszents Hlenlt. word. }
+        lia.
+      }
+      subst logc.
+      rewrite -(take_drop (uint.nat lsnc) logpeer) -Hlogpeer.
+      f_equal.
+      destruct Hlogc as [logtail ->].
+      rewrite take_app_le; last first.
+      { rewrite length_take. clear -Hlsncub. lia. }
+      by rewrite take_idemp.
+    }
+    iMod ("HinvC" with "HinvO") as "_".
+    iAssert (votes_in γ (dom respp') (uint.nat termc) (uint.nat term) (logc ++ ents))%I
+      as "Hvotes'".
+    { iNamed "Hpromise".
+      iNamed "Hvotes".
+      iDestruct (big_sepM_insert_2 with "Hpastd Hdss") as "Hdss'".
+      iFrame "Hdss'".
+      iPureIntro.
+      split.
+      { by apply map_Forall_insert_2. }
+      split.
+      { apply latest_term_before_quorum_with_insert_ge.
+        { by rewrite -not_elem_of_dom -Hdomdss not_elem_of_dom. }
+        { by rewrite /latest_term_nodedec /latest_term_before_nodedec Hlends in Hlatest. }
+        rewrite -latest_term_before_quorum_nodedec_unfold Hlatestq.
+        word.
+      }
+      split.
+      { apply length_of_longest_ledger_in_term_insert_Some_length_ge.
+        { by rewrite -not_elem_of_dom -Hdomdss not_elem_of_dom. }
+        { by rewrite Hacpt. }
+        { destruct (decide (termp = term)) as [-> | Hne].
+          { (* Case: [termp = term]. *)
+            destruct Hcase as [? | Hlonger]; first done.
+            rewrite Hlongestq 2!length_app.
+            lia.
+          }
+          { (* Case: [termp < term]. *)
+            assert (Hltterm : uint.Z termp < uint.Z term) by word.
+            replace (length_of_longest_ledger_in_term _ _) with O; first lia.
+            rewrite /length_of_longest_ledger_in_term /length_of_longest_ledger.
+            replace (omap _ _) with (∅ : gmap u64 ledger).
+            { by rewrite fmap_empty map_fold_empty. }
+            apply map_eq.
+            intros nidx.
+            rewrite lookup_empty lookup_omap.
+            set f := mbind nodedec_to_ledger.
+            set t := uint.nat termc.
+            set p := uint.nat term.
+            unshelve epose proof (latest_term_before_quorum_with_None f dss t p _) as Hnone.
+            { rewrite -latest_term_before_quorum_nodedec_unfold Hlatestq.
+              clear -Hltterm Htermlt.
+              word.
+            }
+            destruct (dss !! nidx) as [dsx |] eqn:Hdsx; last done.
+            simpl.
+            specialize (Hnone _ _ Hdsx).
+            by rewrite /ledger_in_term_with Hnone.
+          }
+        }
+      }
+      split.
+      { apply map_Exists_insert_2_1. by rewrite Hacpt. }
+      { by rewrite 2!dom_insert_L Hdomdss. }
+    }
+    iFrame "Hpx HiscandP HentspP".
+    iFrame "∗ # %".
+    iPureIntro.
+    split; last lia.
+    rewrite dom_insert_L. set_solver.
+  Qed.
 
 End collect.
 
 Section ascend.
   Context `{!heapGS Σ, !paxos_ghostG Σ}.
 
-  Theorem wp_Paxos__ascend (px : loc) nids γ :
+  Theorem wp_Paxos__ascend (px : loc) (nidme : u64) nids γ :
     know_paxos_inv γ nids -∗
-    {{{ own_paxos_nominated px nids γ }}}
+    {{{ own_paxos_nominated px nidme nids γ }}}
       Paxos__ascend #px
-    {{{ RET #(); own_paxos px nids γ }}}.
+    {{{ RET #(); own_paxos px nidme nids γ }}}.
   Proof.
     iIntros "#Hinv" (Φ) "!> Hpx HΦ".
     wp_rec.
@@ -484,8 +779,7 @@ Section ascend.
     wp_if_destruct.
     { iApply "HΦ".
       iFrame "HtermcP HtermlP HiscandP HlogP HentspP".
-      iFrame "∗ # %".
-      admit.
+      by iFrame "∗ # %".
     }
 
     (*@     // Add the longest prefix in the largest term among some quorum (i.e., @*)
@@ -521,7 +815,12 @@ Section ascend.
     { set_solver. }
     { apply Hton. }
     { word. }
-    { (* TODO: prove [safe_base_proposal]. *) admit. }
+    { iFrame "Hvotes".
+      iPureIntro.
+      split; first apply Hdomvts.
+      rewrite /cquorum_size size_dom.
+      word.
+    }
     iMod ("HinvC" with "HinvO") as "_".
 
     (*@     // TODO: Write @px.log and @px.terml to disk.                       @*)
@@ -543,15 +842,87 @@ Section ascend.
     iFrame "Hleader".
     iFrame "HtermcP HtermlP HiscandP".
     iFrame "∗ # %".
+    iModIntro.
+    iSplit.
+    { iClear "Hpreped". by case_decide. }
     iPureIntro.
     split; first done.
     split; first done.
     subst log'.
     rewrite length_app length_take.
     lia.
-  Admitted.
+  Qed.
 
 End ascend.
+
+Section prepare.
+  Context `{!heapGS Σ, !paxos_ghostG Σ}.
+
+  Theorem wp_Paxos__prepare (px : loc) (lsn : u64) (nidme termc terml : u64) nids γ :
+    termc ≠ terml ->
+    {{{ own_paxos_with_termc_terml px nidme termc terml nids γ }}}
+      Paxos__prepare #px #lsn
+    {{{ (entsP : Slice.t) (ents logpeer : list string), RET (#terml, (to_val entsP));
+        own_paxos_with_termc_terml px nidme termc terml nids γ ∗
+        own_slice entsP stringT (DfracOwn 1) ents ∗
+        past_nodedecs_latest_before γ nidme (uint.nat termc) (uint.nat terml) logpeer ∗
+        ⌜drop (uint.nat lsn) logpeer = ents⌝
+    }}}.
+  Proof.
+    iIntros (Hne Φ) "Hpx HΦ".
+    wp_rec.
+
+    (*@ func (px *Paxos) prepare(lsn uint64) (uint64, []string) {               @*)
+    (*@     if uint64(len(px.log)) <= lsn {                                     @*)
+    (*@         return px.terml, make([]string, 0)                              @*)
+    (*@     }                                                                   @*)
+    (*@                                                                         @*)
+    do 2 iNamed "Hpx".
+    case_decide; first done.
+    wp_loadField.
+    iDestruct (own_slice_sz with "Hlog") as %Hsz.
+    wp_apply wp_slice_len.
+    wp_if_destruct.
+    { wp_loadField.
+      wp_apply wp_NewSlice.
+      iIntros (entsP) "Hents".
+      wp_pures.
+      iApply "HΦ".
+      iFrame "Hcand Hleader".
+      iFrame "∗ # %".
+      case_decide; first done.
+      iFrame "Hpreped".
+      iPureIntro.
+      rewrite uint_nat_W64_0 drop_ge /=; [done | lia].
+    }
+
+    (*@     ents := make([]string, uint64(len(px.log)) - lsn)                   @*)
+    (*@     copy(ents, px.log[lsn :])                                           @*)
+    (*@     return px.terml, ents                                               @*)
+    (*@ }                                                                       @*)
+    wp_loadField.
+    wp_apply wp_slice_len.
+    wp_apply wp_NewSlice.
+    iIntros (entsP) "Hents".
+    wp_loadField.
+    iDestruct (own_slice_small_acc with "Hlog") as "[Hlog HlogC]".
+    iDestruct (own_slice_small_acc with "Hents") as "[Hents HentsC]".
+    wp_apply (wp_SliceCopy_SliceSkip_src with "[$Hlog $Hents]").
+    { word. }
+    { rewrite length_replicate /=. word. }
+    iIntros "[Hlog Hents]".
+    iDestruct ("HlogC" with "Hlog") as "Hlog".
+    iDestruct ("HentsC" with "Hents") as "Hents".
+    wp_loadField.
+    wp_pures.
+    iApply "HΦ".
+    iFrame "Hcand Hleader".
+    iFrame "∗ # %".
+    case_decide; first done.
+    by iFrame "Hpreped".
+  Qed.
+
+End prepare.
 
 Section program.
   Context `{!heapGS Σ, !paxos_ghostG Σ}.
